revert erasure to work with unconstrained prophecies

erasure.v
@@ -4,81 +4,34 @@ From iris_io Require Export lang lang_erased.
 From iris.algebra Require Export ofe.
 From stdpp Require Import gmap.
 
-Record Proph_equiv p p' :=
-  { PrA_eq : PrA p = PrA p';
-    PrP_eq :  match PrA_eq in _ = z return z → Stream expr with
-                eq_refl => PrP p end = PrP p' }.
-
-Lemma Proph_equiv_refl p : Proph_equiv p p.
-Proof.
-  unshelve econstructor; eauto.
-Qed.
-
 Definition have_same_proph
            (σ : language.state P_lang) (σ' : language.state PE_lang)
-  := σ.1 = σ'.1 ∧ dom (gset loc) σ.2 = dom (gset loc) σ'.2 ∧
-     ∀ x, x ∈ dom (gset loc) σ.2 →
-          ∃ v v', Proph_equiv v v' ∧
-                  σ.2 !! x = Some v ∧ σ'.2 !! x = Some v'.
+  := σ.1 = σ'.1 ∧ dom (gset loc) σ.2 = σ'.2.
 
-Lemma have_same_proph_refl σ : have_same_proph σ σ.
-Proof.
-  destruct σ as [h p].
-  repeat split; simpl; auto.
-  intros x [v Hv]%elem_of_dom.
-  exists v, v; repeat split; auto using Proph_equiv_refl.
-Qed.
+Definition conjure_prophecies (σ : language.state PE_lang) :
+  language.state P_lang :=
+  match σ with
+    (σh, σp) => (σh,  to_gmap (Sconst UnitV) σp)
+  end.
 
-Program Definition Proph_go_back p p' z w
-           (H : Proph_equiv p (Proph_tail p'))
-           (H' : to_val (Shead (PrP p' z)) = Some w)
-  :=
-{|PrS := {|Shead := w; Stail := PrS p |};
-  PrA := PrA p'; PrP := PrP p'; PrP_ent := PrP_ent p'; PrPvals := PrPvals p' |}.
-Next Obligation.
+Lemma conjure_prophecies_have_same_proph σ :
+  have_same_proph (conjure_prophecies σ) σ.
 Proof.
-  intros p p' z w Pe Pt.
-  destruct p as [pS pA pP pPv pP_ent pPSI].
-  destruct p' as [p'S p'A p'P p'Pv p'P_ent p'PSI].
-  simpl in *.
-  destruct Pe as [Pe1 Pe2]; simpl in *. destruct Pe1; subst.
-  destruct pPSI as [u Hu].
-  destruct (p'Pv u) as [y Hy].
-  destruct (p'Pv z) as [q Hq].
-  destruct (p'P_ent 0 q y) as [x Hx]; auto.
-  rewrite Hq; by eexists.
-  rewrite Hy; by eexists.
-  exists x. rewrite Hx; simpl.
-  destruct y as [yh yt]; simpl in *.
-  rewrite -Hy in Hu; simpl in *.
-  apply proph_to_expr_inj in Hu; subst.
-  destruct q as [qh qt]; simpl in *.
-  rewrite -Hq in Pt; simpl in *.
-  rewrite to_of_val in Pt.
-  by inversion Pt; subst.
-Qed.
-
-Lemma Proph_tail_Proph_go_back p p' z w Heq Heq' :
-  Proph_tail (Proph_go_back p p' z w Heq Heq') = p.
-Proof.
-  destruct p as [pS pA pP pPv pPe pPSI].
-  destruct p' as [p'S p'A p'P p'Pv p'Pe p'PSI].
-  destruct Heq as [Heq1 Heq2].
-  simpl in *.
-  destruct Heq1.
-  match goal with
-    |- ?A = ?B =>
-            eapply (Prohp_eq_simplify A B eq_refl)
-  end; auto.
+  destruct σ; split; first done; simpl.
+  apply mapset.mapset_eq => x; split => Hx.
+  - destruct (decide (x ∈ m)); first done.
+    apply elem_of_dom in Hx. destruct Hx as [y Hy].
+    rewrite lookup_to_gmap option_guard_False //= in Hy.
+  - apply elem_of_dom. rewrite lookup_to_gmap option_guard_True; eauto.
 Qed.
 
 Lemma erased_reachable_reachable th1 h1 th2 σ2:
   rtc (@step PE_lang) (th1, (h1, ∅)) (th2, σ2) →
-  ∀ σ2', have_same_proph σ2' σ2 → rtc (@step P_lang) (th1, (h1, ∅)) (th2, σ2').
+  ∀ σ2', have_same_proph σ2' σ2 →
+         rtc (@step P_lang) (th1, (h1, ∅)) (th2, σ2').
 Proof.
   remember (th1, (h1, ∅)) as cfg.
   remember (th2, σ2) as cfg'.
-  rewrite {2}Heqcfg.
   intros Hrtc.
   revert th1 h1 th2 σ2 Heqcfg Heqcfg'.
   eapply (rtc_ind_r_weak (λ z z', ∀ (th1 : list (language.expr PE_lang)) (h1 : gmap loc val)
@@ -91,9 +44,9 @@ Proof.
                                rtc (@step P_lang) (th1, (h1, ∅)) (th2, σ2')));
   last eauto.
   - intros x th1 h1 th2 σ2 Heqcfg Heqcfg'; simplify_eq.
-    intros [σ2 σ2p] [Hh [Hsp _]]; simpl in *.
-    rewrite dom_empty_L in Hsp. apply dom_empty_inv_L in Hsp. rewrite Hsp.
-    rewrite Hh.  econstructor.
+    intros [σ2 σ2p] [Hh Hsp]; simpl in *.
+    rewrite Hh. rewrite (dom_empty_inv_L (D := gset loc) σ2p); last done.
+    econstructor.
   - intros x y z Hxy Hyz IH th1 h1 th2 σ2 Heqcfg Heqcfg' σ2' Hsp;
       simplify_eq; simpl in *.
     destruct y as [yh yp].
@@ -103,86 +56,47 @@ Proof.
       try (eapply rtc_r; first (by eapply IH; eauto); by repeat (econstructor; eauto)).
     all: destruct σ2' as [σ2'h σ2'p]; destruct Hsp as [Hsp1 Hsp2]; simpl in *; simplify_eq.
     + eapply (rtc_r _ (_ ++ fill K (Alloc _) :: _, (σ, σ2'p)));
-        [unshelve eapply (IH _ _ _ (_, σp) _ _ (σ, σ2'p)); eauto; split; simpl; eauto|
+        [unshelve eapply (IH _ _ _ (_, _) _ _ (σ, σ2'p)); eauto; split; simpl; eauto|
          repeat (econstructor; eauto)].
     + match goal with A : ?X.1 !! _ = _ |- _ => destruct X as [σmh σmp]; simpl in * end.
       eapply (rtc_r _ (_ ++ fill K (Load (Loc _)) :: _, (_, σ2'p)));
         [unshelve eapply (IH _ _ _ (σmh, σmp) _ _ (_, σ2'p)); eauto; split; simpl; eauto|
          repeat (econstructor; eauto)].
     + eapply (rtc_r _ (_ ++ fill K (Store (Loc _) _) :: _, (_, σ2'p)));
-        [unshelve eapply (IH _ _ _ (_, σp) _ _ (_, σ2'p)); eauto; split; simpl; eauto|
+        [unshelve eapply (IH _ _ _ (_, _) _ _ (_, σ2'p)); eauto; split; simpl; eauto|
          repeat (econstructor; eauto)].
     + match goal with A : ?X.1 !! _ = _ |- _ => destruct X as [σmh σmp]; simpl in * end.
       eapply (rtc_r _ (_ ++ fill K (CAS (Loc _) _ _) :: _, (_, σ2'p)));
-        [unshelve eapply (IH _ _ _ (_, σmp) _ _ (_, σ2'p)); eauto; split; simpl; eauto|
+        [unshelve eapply (IH _ _ _ (_, _) _ _ (_, σ2'p)); eauto; split; simpl; eauto|
          repeat (econstructor; eauto)].
     + eapply (rtc_r _ (_ ++ fill K (CAS (Loc _) _ _) :: _, (_, σ2'p)));
-        [unshelve eapply (IH _ _ _ (_, σp) _ _ (_, σ2'p)); eauto; split; simpl; eauto|
+        [unshelve eapply (IH _ _ _ (_, _) _ _ (_, σ2'p)); eauto; split; simpl; eauto|
          repeat (econstructor; eauto)].
-    + destruct Hsp2 as [Hsp21 Hsp22].
-      assert (dom (gset loc) (delete (fresh (dom (gset loc) σp)) σ2'p)
-                = dom (gset loc) σp) as Hfr.
-      { rewrite dom_delete_L Hsp21 dom_insert_L difference_union_distr_l_L
-                  difference_diag_L left_id_L difference_disjoint_L //=.
-          apply disjoint_singleton_r, is_fresh. }
-      eapply (rtc_r _ (_ ++ fill K (Create_Pr A P) :: _, (σ, delete (fresh (dom (gset loc) σp)) σ2'p)));
-        [unshelve eapply (IH _ _ _ (σ, σp) _ _ (_, _)); eauto; simpl; eauto|
+    + assert (({[fresh σp]} ∪ σp) ∖ {[fresh σp]} = σp) as Hfr.
+      { rewrite difference_union_distr_l_L difference_diag_L left_id_L.
+        apply difference_disjoint_L.
+        symmetry. apply disjoint_singleton_l, is_fresh. }
+      eapply (rtc_r _ (_ ++ fill K (Create_Pr) :: _, (_, delete (fresh σp) σ2'p)));
+        [unshelve eapply (IH _ _ _ (_, _) _ _ (_, _)); eauto; split; simpl; eauto|
          repeat (econstructor; eauto)].
-      * repeat split; auto; simpl.
-        intros x Hx. rewrite dom_delete_L in Hx.
-        apply elem_of_difference in Hx; destruct Hx as [Hx1 Hx2].
-        edestruct Hsp22 as (v1 & v2 & Hvv & Hv1 & Hv2); eauto.
-        apply not_elem_of_singleton in Hx2.
-        exists v1, v2; split; auto. split.
-        ++ rewrite lookup_delete_ne; auto.
-        ++ rewrite lookup_insert_ne in Hv2; auto.
-      * destruct (elem_of_dom (D := gset loc) σ2'p (fresh (dom (gset loc) σp))) as [[p Hp]].
-        { rewrite Hsp21 dom_insert.  by apply elem_of_union_l, elem_of_singleton. }
-        simpl.
-        replace σ2'p with (<[fresh (dom (gset loc) (delete (fresh (dom (gset loc) σp)) σ2'p)) := p]> (delete (fresh (dom (gset loc) σp)) σ2'p)) at 2; last first.
-        { rewrite Hfr. by rewrite insert_delete insert_id. }
-        rewrite -{2}Hfr.
-        destruct p as [str sA sP sSI].
-        destruct (Hsp22 (fresh (dom (gset loc) σp))) as (v1 & v2 & Hvv & Hv1 & Hv2); eauto.
-        rewrite lookup_insert in Hv2. rewrite Hp in Hv1.
-        inversion Hv1; inversion Hv2; simplify_eq.
-        destruct Hvv as [Hvv1 Hvv2]; simpl in *.
-        destruct Hvv1; simplify_eq.
-        apply Create_PrS.
-    + destruct Hsp2 as [Hsp21 Hsp22].
-      assert (∃ str, σ2'p !! l = Some str) as [str Hstr].
-      { apply (elem_of_dom (D := gset loc)).
-        rewrite Hsp21 dom_insert. by apply elem_of_union_l, elem_of_singleton. }
-      destruct (Hsp22 l) as (v1 & v2 & Hvv & Hv1 & Hv2); first apply elem_of_dom; eauto.
-      rewrite Hv1 in Hstr; inversion Hstr; subst; clear Hstr.
-      rewrite lookup_insert in Hv2; inversion Hv2; subst; clear Hv2.
+      * by rewrite (dom_delete_L (D := gset loc)) Hsp2 Hfr.
+      * destruct (elem_of_dom (D := gset loc) σ2'p (fresh σp)) as [[str Hstr]].
+        { rewrite Hsp2. by apply elem_of_union_l, elem_of_singleton. }
+        replace σ2'p with (<[fresh (dom (gset loc) (delete (fresh σp) σ2'p)) := str]> (delete (fresh σp) σ2'p)) at 2; last first.
+        { rewrite dom_delete_L Hsp2 Hfr insert_delete. by apply insert_id. }
+        rewrite -{2}Hfr -Hsp2 -dom_delete_L.
+        econstructor.
+    + assert (∃ str, σ2'p !! l = Some str) as [str Hstr]
+          by by apply (elem_of_dom (D := gset loc)).
       eapply (rtc_r _ (_ ++ fill K (Assign_Pr (Pr _) _) :: _,
-                       (_, <[l:= (Proph_go_back _ _ _ _ Hvv H0)]> σ2'p)));
-        [unshelve eapply (IH _ _ _ (_, σp) _ _ (_, _)); eauto; split; simpl; eauto|
+                       (_, <[l:={| Shead := v; Stail := str|}]> σ2'p)));
+        [unshelve eapply (IH _ _ _ (_, _) _ _ (_, _)); eauto; split; simpl; eauto|
          repeat (econstructor; eauto)].
-      * assert (dom (gset loc) (<[l:=p]> σ2'p) = dom (gset loc) σ2'p) as Hσ2'p.
-        { rewrite dom_insert_L Hsp21 dom_insert_L assoc_L idemp_L.
-           rewrite subseteq_union_1_L //.
-           apply elem_of_subseteq_singleton, elem_of_dom; eauto. }
-        split; auto.
-        ++ rewrite dom_insert_L Hsp21 dom_insert_L assoc_L idemp_L.
-           rewrite subseteq_union_1_L //.
-           apply elem_of_subseteq_singleton, elem_of_dom; eauto.
-        ++ intros x. rewrite dom_insert_L. rewrite dom_insert_L in Hσ2'p.
-           rewrite Hσ2'p. intros Hx.
-           destruct (Hsp22 _ Hx) as (w1 & w2 & Hww & Hw1 & Hw2).
-           destruct (decide (x = l)); subst.
-           -- eexists (Proph_go_back str p _ _ Hvv H0), p; repeat split; auto;
-                last by rewrite lookup_insert.
-              unshelve econstructor; auto.
-           -- exists w1, w2; repeat split; auto; rewrite -?Hw2 lookup_insert_ne //.
-      * replace σ2'p with (<[l:= (Proph_tail (Proph_go_back str p _ _ Hvv H0))]>(<[l:= Proph_go_back str p _ _ Hvv H0]> σ2'p)) at 2; last first.
-        { apply map_eq => i. destruct (decide (i = l)); subst.
-          - rewrite lookup_insert Hv1. f_equal.
-            apply Proph_tail_Proph_go_back.
-          - do 2 rewrite lookup_insert_ne //=. }
-        econstructor; eauto.
-        by rewrite lookup_insert.
+      * rewrite dom_insert_L. by apply subseteq_union_1_L, elem_of_subseteq_singleton.
+      * replace σ2'p with (<[l:= Stail {| Shead := v; Stail := str |}]>(<[l:={| Shead := v; Stail := str |}]> σ2'p)) at 2; last first.
+        { rewrite /= insert_insert. by apply insert_id. }
+        econstructor; auto.
+        rewrite lookup_insert //.
 Qed.
 
 Definition safe e :=
@@ -195,32 +109,33 @@ Definition erased_safe e :=
     rtc (@step PE_lang) ([e], (∅, ∅)) (th2, σ2) →
     ∀ e, e ∈ th2 → AsVal e ∨ reducible e σ2.
 
-Lemma reducible_erase_reducible e σ :
-  @language.reducible P_lang e σ →
-  @language.reducible PE_lang e σ.
+Lemma reducible_erase_reducible e σ σ' :
+  have_same_proph σ σ' →
+  reducible e σ →
+  @language.reducible PE_lang e σ'.
 Proof.
-  intros (e'&σ2&efs&Hrd); simpl in *.
+  intros Hsp (e'&σ2&efs&Hrd); simpl in *.
   inversion Hrd as [K e1' e2' ? ? Hhrd]; simpl in *; subst.
-  destruct σ as [σh σp]; simpl in *; simplify_eq.
-  inversion Hhrd; subst;
-    try (solve [unshelve (repeat econstructor; eauto)]).
+  destruct σ as [σh σp]; destruct σ' as [σ'h σ'p];
+    destruct Hsp as [? ?]; simpl in *; simplify_eq.
+  inversion Hhrd; subst; try (unshelve (repeat econstructor; eauto); fail).
   + match goal with A : is_Some _ |- _ => destruct A as [? ?] end.
     repeat econstructor; eauto.
-  + do 3 eexists. econstructor; eauto. unshelve econstructor; eauto.
-  + destruct (PrSI p) as [x Hx].
-    do 3 eexists. econstructor; eauto. econstructor; eauto.
-    by apply of_to_val in H6; rewrite -H6.
-  + do 3 eexists. econstructor; eauto. unshelve econstructor.
-    constructor.
+  + repeat econstructor; eauto.
+    apply elem_of_dom; eauto.
+  + repeat econstructor; eauto.
+    apply elem_of_dom; eauto.
+  + by unshelve (repeat econstructor).
 Qed.
 
 Lemma soundness_prophecies e :
   safe e → erased_safe e.
 Proof.
   intros Hs th2 σ2 Hrtc re Hre.
-  assert (rtc step ([e], (∅, ∅)) (th2, σ2)) as Hrtc'.
+  assert (rtc step ([e], (∅, ∅)) (th2, conjure_prophecies σ2)) as Hrtc'.
   { eapply erased_reachable_reachable;
-      eauto using have_same_proph_refl. }
+      eauto using conjure_prophecies_have_same_proph. }
   edestruct Hs as [?|Hred]; eauto.
-  right. by eapply reducible_erase_reducible.
+  right. eapply reducible_erase_reducible;
+           eauto using conjure_prophecies_have_same_proph.
 Qed.
